Json.Parser.fst
@@ -1,0 +1,182 @@
+module Json.Parser
+
+open FStar.Char
+open FStar.UInt32
+open FStar.String
+open FStar.Option
+open FStar.List.Tot
+open FStar.List.Tot.Properties
+open Json.Grammar
+
+module G = Json.Grammar
+module Option = FStar.Option
+module Char = FStar.Char
+module U32 = FStar.UInt32
+module String = FStar.String
+
+type char = Char.char
+
+let str_to_char (s: string{String.strlen s == 1}) : char = let c::_ = String.list_of_string s in c
+
+// This type holds a successful parsing of a string which is decomposed in a parsed prefix and the remainder of the string
+type parser_result a = {
+  result: a;
+  remainder: string;
+}
+
+type nonempty_str = s:string{match String.list_of_string s with | c::tail -> true | _ -> false }
+
+// Utility lemma to decompose a string into two list of characters
+let str_decompose (s: string) (c1 c2: list char) : 
+  Lemma 
+  (requires (String.list_of_string s == c1 @ c2))
+  (ensures (s == (String.string_of_list c1) ^ (String.string_of_list c2))) = 
+  let c1_str = String.string_of_list c1 in
+  let c2_str = String.string_of_list c2 in
+  // s == string_of_list(list_of_string(s))
+  String.string_of_list_of_string s;
+  //   == string_of_list([c]) + string_of_list(tail) 
+  String.list_of_concat c1_str c2_str;
+  String.list_of_string_of_list c1;
+  String.list_of_string_of_list c2;
+  String.string_of_list_of_string (c1_str ^ c2_str)
+
+// Utility lemma proving that chopping off the first character of a non-empty string decreases the string's length
+let str_tail_decrease (s: nonempty_str) : 
+  Lemma 
+  (ensures (
+    let c::tail = String.list_of_string s in 
+    let tail_str = String.string_of_list tail in
+    String.strlen tail_str < String.strlen s
+    )
+  ) =
+  let c::tail = String.list_of_string s in
+  // list_of_string s = [c] + tail
+  assert(String.list_of_string s == [c] @ tail);
+  // len(tail) = len(tail_str)
+  String.list_of_string_of_list tail
+  // len(s) = len(append([c], tail)) = len([c]) + len(tail)
+  // len(tail_str) < len(s)
+
+let list_of_string_eq (s1 s2: string): Lemma (requires s1 == s2) (ensures String.list_of_string s1 == String.list_of_string s2) = ()
+
+// Utility lemma proving that string concatenation is associative
+let str_concat_assoc (s1 s2 s3: string) : Lemma (ensures ((s1 ^ s2) ^ s3) == (s1 ^ (s2 ^ s3))) =
+  let s1_chars = String.list_of_string s1 in
+  let s2_chars = String.list_of_string s2 in
+  let s3_chars = String.list_of_string s3 in
+  // (s1 ^ s2) ^ s3 == string_of_list(list_of_string((s1 ^ s2) ^ s3))
+  string_of_list_of_string ((s1 ^ s2) ^ s3);
+  // list_of_string(s1 ^ s2) == list_of_string(s1) @ list_of_string(s2)
+  list_of_concat s1 s2;
+  // list_of_string((s1 ^ s2) ^ s3) == list_of_string(s1 ^ s2) @ list_of_string(s3)
+  list_of_concat (s1 ^ s2) s3;
+  FStar.List.Tot.Properties.append_assoc s1_chars s2_chars s3_chars;
+  list_of_concat s1 (s2 ^ s3);
+  list_of_concat s2 s3;
+  string_of_list_of_string (s1 ^ (s2 ^ s3))
+
+
+let rec parse_json_ws (s: string) : Tot (parser_result G.json_ws) (decreases (String.strlen s)) = 
+  match String.list_of_string s with
+  | [] -> { // Empty string
+    result = G.NoWhitespace;
+    remainder = s;
+  }
+  | c::tail -> 
+    let is_whitespace = (c = G.char_from_codepoint 0x20) || (c = G.char_from_codepoint 0x0A) || (c = G.char_from_codepoint 0x0D) || (c = G.char_from_codepoint 0x09) in
+    if is_whitespace then
+      let tail_str = String.string_of_list tail in
+      // Prove termination of recursive call
+      str_tail_decrease s;
+      let tail_parse = parse_json_ws tail_str in
+      {
+        result = G.Whitespace c tail_parse.result;
+        remainder = tail_parse.remainder;
+      }
+    else
+      { 
+        result = G.NoWhitespace;
+        remainder = s;
+      }
+
+
+
+// Prove correctness of whitespace parsing
+let prepend_empty_is_identity (s: string) : Lemma (ensures ("" ^ s) == s) =
+    // list_of_string("" + s) = list_of_string("") @ list_of_string(s) = list_of_string(s) 
+    list_of_concat "" s;
+    assert(String.list_of_string ("" ^ s) == String.list_of_string s);
+    // "" + s = string_of_list(list_of_string("" + s)) = string_of_list(list_of_string(s)) == s
+    String.string_of_list_of_string ("" ^ s);
+    String.string_of_list_of_string s
+
+let rec parse_json_ws_soundness (s: string) :
+  Lemma 
+  (ensures (
+    let parsed = parse_json_ws s in
+    s == (G.render_json_ws parsed.result) ^ parsed.remainder
+  ))
+  (decreases (String.strlen s)) =
+  match String.list_of_string s with
+    | [] -> 
+      // By definition of parse_json_ws, it suffices to show s == "" + s
+      prepend_empty_is_identity s
+    | c::tail -> 
+      let is_whitespace = (c = G.char_from_codepoint 0x20) || (c = G.char_from_codepoint 0x0A) || (c = G.char_from_codepoint 0x0D) || (c = G.char_from_codepoint 0x09) in
+      if is_whitespace then
+        let tail_str = String.string_of_list tail in
+        let tail_parse = parse_json_ws tail_str in
+        // Prove s == (c + tail_parse.result) + tail_parse.remainder
+        list_of_string_of_list [c];
+        //         == c + (tail_parse.result + tail_parse.remainder)
+        str_concat_assoc (G.char_to_str c) (G.render_json_ws tail_parse.result) tail_parse.remainder;
+        //         == c + tail_str [by induction]
+        // Prove termination of recursive call
+        str_tail_decrease s;
+        parse_json_ws_soundness tail_str;
+        // Prove s == string_of_list([c]) + tail_str
+        str_decompose s [c] tail
+      else
+        prepend_empty_is_identity s
+
+
+let rec parse_json_ws_completeness (ws: G.json_ws) :
+  Lemma
+  (ensures (
+    let rendered_ws = G.render_json_ws ws in
+    let parsed = parse_json_ws rendered_ws in
+    ws == parsed.result /\ parsed.remainder == ""
+  )) =
+  let rendered_ws = G.render_json_ws ws in
+  let parsed = parse_json_ws rendered_ws in
+  match ws with
+  | G.NoWhitespace -> ( 
+    // Force F* into recognizing that match statement of parsing takes the empty list branch
+    list_of_string_eq rendered_ws "";
+    assert(parsed.result == NoWhitespace);
+    assert(parsed.remainder == "")
+  )
+  | G.Whitespace c ws' -> (
+    let rendered_ws' = render_json_ws ws' in
+    // rendered_ws = c + render(ws')
+    assert(rendered_ws == G.char_to_str c ^ rendered_ws');
+    // list_of_string(rendered_ws) = [c] + list_of_string(render(ws'))
+    String.list_of_concat (G.char_to_str c) rendered_ws';
+    String.list_of_string_of_list [c];
+    // parsed = {result = Whitespace c parse(render(ws')).result; remainder = parse(render(ws')).remainder}
+    //        = {result = Whitespace c ws').result; remainder = ""}
+    match String.list_of_string rendered_ws with
+      // The naming of c is not ambiguous as they are (provably) the same c
+      | c::parse_tail -> (
+        let parse_tail_str = String.string_of_list parse_tail in
+        assert(parse_tail == String.list_of_string rendered_ws');
+        String.string_of_list_of_string rendered_ws';
+        assert(parse_tail_str == rendered_ws');
+        // Perform induction on parse_tail which is basically ws'
+        parse_json_ws_completeness ws';
+        assert(parsed.remainder == "");
+        assert(parsed.result == Whitespace c ws');
+        ()
+      )
+  )
